Simplified the direct semantics.

withtop/Proofs/semantics/SemanticsSimpl.v
@@ -43,13 +43,8 @@ Inductive typing : ST.context PTyp -> PExp -> PTyp -> Prop :=
                WFTyp B ->
                typing Gamma t B.
 
-Inductive Value : PExp -> Prop :=
-  | VLit : forall n, Value (PLit n)
-  | VLam : forall e A B, Value (PAnn CT (PLam e) (Fun A B))
-  | VMerge : forall v1 v2, Value v1 -> Value v2 -> Value (PMerge v1 v2).
-
 Inductive In : PExp -> PTyp -> Prop :=
-  | InInt : forall n, In (PLit n) PInt
+  | InInt : forall n, In (PAnn CT (PLit n) PInt) PInt
   | InFun : forall e A B, In (PAnn CT (PLam e) (Fun A B)) (Fun A B)
   | InAnd : forall v1 v2 A B, In v1 A ->
                          In v2 B ->
@@ -94,73 +89,61 @@ Inductive bidityping : ST.context PTyp -> PExp -> Dir -> PTyp -> Prop :=
                 WFTyp B ->
                 bidityping Gamma t Chk B.
 
-Inductive IsFun : PTyp -> Prop := IsF : forall A B, IsFun (Fun A B).
-
 Inductive red : PExp -> PExp -> Prop :=
+  | Red_Int : forall n, red (PLit n) (PAnn CT (PLit n) PInt)
   | Red_App1 : forall e1 e2 e3,
                  red e1 e3 ->
                  red (PApp e1 e2) (PApp e3 e2)
   | Red_App2 : forall e1 e2 v A B,
-                 Value v ->
-                 not (In e1 A) ->
+                 ~ (In e1 A) ->
                  In v (Fun A B) ->
-                 red (PAnn CT e1 A) e2 ->
+                 red (PAnn CT e1 A) (PAnn CT e2 A) ->
                  red (PApp v e1) (PApp v e2)
   | Red_App3 : forall A B e v,
-                 Value v ->
                  In v A -> 
                  red (PApp (PAnn CT (PLam e) (Fun A B)) v)
                      (PAnn CT (open_source e v) B)
   | Red_Merge1 : forall e1 e2 e3,
                    red e1 e3 ->
                    red (PMerge e1 e2) (PMerge e3 e2)
-  | Red_Merge2 : forall e1 e2 v,
-                   Value v ->
+  | Red_Merge2 : forall e1 e2 v A B,
+                   In v (And A B) ->
                    red e1 e2 ->
                    red (PMerge v e1) (PMerge v e2)
-  | Red_Ann : forall e1 e2 A,
-                red e1 e2 ->
-                red (PAnn CT e1 A) (PAnn CT e2 A)
-  | Red_Ann2 : forall A B v,
-                 Value v ->
+  | Red_Ann1 : forall e1 e2 A,
+                 ~ (In (PAnn CT e1 A) A) ->
+                 ~ In e1 A ->
+                 red e1 e2 ->
+                 red (PAnn CT e1 A) (PAnn CT e2 A)
+  | Red_Ann2 : forall A v,
                  In v A ->
-                 ~ (IsFun A) -> 
-                 red (PAnn CT (PAnn CT v A) B) (PAnn CT v B)
-  | Red_Ann2Abs :
+                 red (PAnn CT v A) v
+  | Red_Ann3Abs :
       forall e A B C D,
+        Fun A B <> Fun C D ->
         red (PAnn CT (PAnn CT (PLam e) (Fun A B)) (Fun C D))
             (PAnn CT (PLam (PAnn CT (PApp (PAnn CT (PLam e) (Fun A B))
                                           (PAnn CT (PBVar 0) A)) D))
                   (Fun C D))
-  | Red_Ann3 : forall A v,
-                 Value v ->
-                 In v A ->
-                 ~ (IsFun A) -> 
-                 red (PAnn CT v A) v
   | Red_Ann4 : forall v1 v2 A B C,
                     Sub B A ->
                     Atomic A ->
-                    Value v1 ->
-                    Value v2 ->
                     In (PMerge v1 v2) (And B C) ->
                     red (PAnn CT (PMerge v1 v2) A)
                         (PAnn CT v1 A)
   | Red_Ann5 : forall v1 v2 A B C,
                  Sub C A ->
                  Atomic A ->
-                 Value v1 ->
-                 Value v2 ->
                  In (PMerge v1 v2) (And B C) ->
                  red (PAnn CT (PMerge v1 v2) A)
                      (PAnn CT v2 A)
   | Red_Ann6 : forall v A B C D,
-                 Value v ->
                  In v (And C D) ->
                  (And C D) <> (And A B) ->
                  red (PAnn CT v (And A B))
                      (PMerge (PAnn CT v A) (PAnn CT v B)).
 
-Hint Constructors typing bidityping Value In WFTyp red IsFun.
+Hint Constructors typing bidityping In WFTyp red.
 
 (** Soundness and Completeness wrt to the elaborating biditypecheker **)
 
@@ -251,8 +234,8 @@ Proof. intros Gamma t A B m1 m2 Htyping; dependent induction Htyping; eauto. Qed
 
 (** Properties mixing "Sub", "In" and the type-system. **)
 
-Theorem In_Ann_inv : forall v A B, Value v -> In (PAnn CT v A) B -> A = B.
-Proof. intros v A B H1 H2; dependent induction H2; auto. Qed.
+Theorem In_Ann_inv : forall v A B, In (PAnn CT v A) B -> A = B.
+Proof. intros v A B H1; dependent induction H1; auto. Qed.
 
 (*Hint Resolve bityping_ann_sub bityping_ann.*)
 Hint Resolve In_Ann_inv.
@@ -281,7 +264,6 @@ Proof.
   assert (HSub : Sub A B) by eauto.
   generalize dependent A.
   induction Htyping; intros; try now inversion HIn.
-  - inversion HIn; auto.
   - apply invAndS1 in HSub. destruct HSub.
     inversion HIn; subst.
     assert (Ha1 : Sub A1 A) by eauto.
@@ -379,40 +361,38 @@ Proof.
   induction Hred; intros; try now (dependent induction Htyping; subst; eauto).
   - (* R_App2 *)
     dependent induction Htyping; subst; eauto; clear IHHtyping1 IHHtyping2.
-    inversion H1; subst; inversion Htyping1; subst.
+    inversion H0; subst; inversion Htyping1; subst.
     apply ATyApp' with (A := A0); auto.
+    assert (Ha : bidityping Gamma (PAnn CT e1 A0) Inf A0) by eauto.
+    apply IHHred in Ha; inversion Ha; now subst.
   - (* R_App3 *)
     dependent induction Htyping; subst; eauto.
     clear IHHtyping1 IHHtyping2.
     inversion Htyping1; subst.
     apply ATyAnnCT'; clear Htyping1.
     apply open_body_bityping with (A := A0); eauto.
-    inversion H5; subst; eauto.
-    inversion H1.
+    inversion H4; subst; eauto.
+    inversion H0.
     dependent induction Htyping2; subst; eauto.
     inversion H2.
   - (* R_Ann2 *)
     dependent induction Htyping; eauto; subst; clear IHHtyping.
-    inversion Htyping; subst.
-    inversion H2; subst.
-    inversion H2; subst.
-    dependent induction H8; eauto.
-    clear H6.
-    exfalso; now apply H1.
+    dependent induction Htyping; eauto.
+    inversion H2. 
   - (* R_AnnAbs *)
     dependent induction Htyping; subst; eauto; clear IHHtyping.
     inversion Htyping; subst.
-    inversion H; subst.
-    inversion H1; subst.
+    inversion H0; subst.
+    inversion H2; subst.
     apply ATyAnnCT'.     
     apply_fresh ATyLam' as x; auto.
     unfold open_source; simpl.
     assert (Ha : Sub D D) by apply reflex; destruct Ha.
     assert (Ha : WFTyp A) by
-        (now assert (Ha := bityping_wf _ _ _ _ H); inversion Ha).
+        (now assert (Ha := bityping_wf _ _ _ _ H0); inversion Ha).
     eapply ATySub' with (A := D); eauto 2.
     apply ATyAnnCT'.
-    inversion H0; subst; clear H0.
+    inversion H1; subst; clear H1.
     eapply ATySub' with (A := B); eauto 2.
     eapply ATyApp' with (A := A).
     + apply ATyAnnCT'.
@@ -431,26 +411,20 @@ Proof.
       apply ST.Ok_push; eauto.
       ST.not_in_L x.
       now left.
-  - (* R_Ann3 *)
-    dependent induction Htyping; subst; eauto; clear IHHtyping.
-    dependent induction Htyping; subst; eauto.
-    exfalso; now apply H4.
   - (* R_Ann4 *)
     dependent induction Htyping; subst; eauto; clear IHHtyping.
     destruct H.
     inversion Htyping; subst.
-    inversion H3; inversion H4; subst.
-    eauto.
+    inversion H2; inversion H1; subst; eauto.
   - (* R_Ann5 *)
     dependent induction Htyping; subst; eauto; clear IHHtyping.
     destruct H.
     inversion Htyping; subst.
-    inversion H3; inversion H4; subst.
-    eauto.
+    inversion H2; inversion H1; subst; eauto.
   - (* R_Ann6 *)
     dependent induction Htyping; subst; eauto; clear IHHtyping.
     inversion Htyping; subst.
-    inversion H0; subst.
+    inversion H2; subst; try now inversion H5.
     assert (Ha : WFTyp (And A B)) by eauto; inversion Ha; subst.
     assert (Ha2 : Sub A0 A) by eauto.
     assert (Ha3 : Sub A0 B) by eauto.
@@ -458,24 +432,25 @@ Proof.
     apply ATyMerge'; eauto.
 Qed.
 
-(** Theorem 2. **)
+(** Theorem 2. Reduction is deterministic **)
 
 Hint Extern 1 =>
   match goal with
-    | [ H : ~ IsFun (Fun ?A ?B) |- _ ] => exfalso; now apply H
     | [ H : red (PLam ?e2) ?e1 |- _ ] => inversion H
+    | [ H : In (PLam ?e) ?A |- _ ] => inversion H
+    | [ H : In (PInt ?e) ?A |- _ ] => inversion H
   end. 
 
-Lemma value_not_red : forall e1 e2, Value e1 -> red e1 e2 -> False.
+Lemma value_not_red : forall e1 e2 A, In e1 A -> red e1 e2 -> False.
 Proof.
-  intros e1 e2 Hvalue Hred.
-  induction Hred; inversion Hvalue; subst; auto.
+  intros e1 e2 A Hin Hred. generalize dependent A.
+  induction Hred; intros; inversion Hin; subst; eauto; inversion H.
 Qed.
 
 Hint Extern 1 =>
   match goal with
-    | [ H1 : Value (?e1),
-        H2 : red ?e1 ?e2 |- _ ] => exfalso; apply (value_not_red _ _ H1 H2)
+    | [ H1 : In ?e1 ?A,
+        H2 : red ?e1 ?e2 |- _ ] => exfalso; apply (value_not_red _ _ _ H1 H2)
   end. 
 
 Lemma In_unique : forall v A B, In v A -> In v B -> A = B.
@@ -487,32 +462,22 @@ Proof.
   now subst.
 Qed.
 
-Lemma In_value : forall v A, In v A -> Value v.
-Proof. intros v A H; induction H; auto. Qed.
-
 Hint Rewrite In_unique.
-Hint Resolve In_value.
-
-Lemma value_ann_red_refl :
-  forall v A, In v A -> ~ IsFun A -> red (PAnn CT v A) v.
-Proof. intros v A Hin Hfun; inversion Hin; subst; eauto. Qed.
-
-Lemma value_ann_red_eq :
-  forall v A e, In v A -> ~ IsFun A -> red (PAnn CT v A) e -> v = e.
+    
+Lemma value_ann_red_id :
+  forall v A e, In v A -> red (PAnn CT v A) e -> v = e.
 Proof.
-  intros v A e Hin Hfun Hred.
+  intros v A e Hin Hred.
   dependent induction Hred; eauto.
-  - apply In_value in Hin; auto.
-  - inversion Hin; subst; auto.
+  - inversion Hin; subst; exfalso; now apply H.
   - inversion Hin; subst; inversion H0.
   - inversion Hin; subst; inversion H0.
   - inversion Hin; subst.
-    assert (And C D = And A0 B) by (eapply In_unique; eauto).
-    inversion H2; subst; contradiction.
+    assert (Ha : And C D = And A0 B) by (eapply In_unique; eauto).
+    inversion Ha; subst; contradiction.
 Qed.
 
-Hint Resolve value_ann_red_refl.
-Hint Rewrite value_ann_red_eq.
+Hint Rewrite value_ann_red_id.
 
 Theorem red_unique :
   forall e1 e2, red e1 e2 -> forall e3, red e1 e3 -> e2 = e3.
@@ -520,78 +485,75 @@ Proof.
   intros e1 e2 Hred.
   induction Hred; intros.
   - inversion H; subst; auto.
+  - inversion H; subst; auto.
     + apply IHHred in H3; now subst.
     + inversion Hred; subst; auto.
-  - inversion H1; subst.
-    inversion H2; subst; auto.
-    + inversion H7; subst; apply IHHred in H9; now subst.
+  - inversion H0; subst.
+    inversion H1; subst; auto.
+    + assert (Ha : Fun A B = Fun A0 B0) by eauto; inversion Ha; subst.
+      apply IHHred in H7; inversion H7; now subst.
     + contradiction.
-  - inversion H1; subst; auto.
-    + inversion H5; subst; auto.
-    + inversion H6; subst; contradiction.
+  - inversion H0; subst; auto.
+    + inversion H4; subst; auto. 
+    + inversion H4; subst; contradiction.
   - inversion H; subst; auto.
     + apply IHHred in H3; now subst.
   - inversion H; subst.
-    + inversion H0; subst; auto.
-      apply IHHred in H5; now subst.
-    + inversion H0; subst; auto.
-      apply IHHred in H5; now subst.
-    + inversion H0; subst; auto.
-      apply IHHred in H7; now subst.
-  - inversion H; subst; auto; try now (inversion Hred; subst; auto).
-    + apply IHHred in H3; now subst.
-    + assert (Ha : red (PAnn CT v A0) v) by eauto.
-      apply IHHred in Ha; now subst.
-  - inversion H2; subst; auto.
-    assert (v = e2) by (eapply value_ann_red_eq; eauto); now subst.
-    inversion H5; subst; auto.
-    inversion H5; subst; auto.
-  - inversion H; subst; auto.
-    inversion H3; subst; auto.
-  - eapply value_ann_red_eq; eauto.
-  - inversion H4; subst; auto.
-    inversion H8; subst; auto.
-    inversion H8; subst. inversion H0.
+    inversion H; inversion H0; subst; auto.
+    apply IHHred in H15; now subst.
+  - inversion H1; subst; auto; try now (inversion Hred; subst; auto).
+    + apply IHHred in H7; now subst.
+  - inversion H0; subst; auto.
+    assert ((Fun A0 B) = (Fun C D)) by eauto; contradiction.
+    inversion H; subst; inversion H4.
+    inversion H; subst; inversion H4.
+    assert (Ha : And C D = And A0 B) by (eapply In_unique; eauto); inversion Ha; subst.
+    exfalso; now apply H5.
+  - inversion H0; subst; auto.
+    inversion H6; subst; auto.
+    assert ((Fun A B) = (Fun C D)) by eauto; contradiction.
+  - inversion H1; subst.
+    dependent induction H2; subst; auto.
+    inversion H2; subst; inversion H0.
     assert (Ha : And B C = And B0 C0) by (eapply In_unique; eauto); inversion Ha; subst.
-    inversion H3; subst.
     assert (Ha1 : ~ (Sub C0 A /\ Sub B0 A)) by eauto.
     exfalso; apply Ha1; split; assumption.
     inversion H0.
-  - inversion H4; subst; auto.
-    inversion H8; subst; auto.
-    inversion H8; subst. inversion H0.
+  - inversion H1; subst.
+    dependent induction H2; subst; auto.
+    inversion H2; subst; inversion H0.
     assert (Ha : And B C = And B0 C0) by (eapply In_unique; eauto); inversion Ha; subst.
-    inversion H3; subst.
     assert (Ha1 : ~ (Sub C0 A /\ Sub B0 A)) by eauto.
     exfalso; apply Ha1; split; assumption.
     inversion H0.
-  - inversion H0; subst; inversion H; subst.
-    inversion H2; subst; auto.
+  - inversion H; subst.
+    inversion H1; subst; auto.
     assert (Ha : And C D = And A B) by (eapply In_unique; eauto); inversion Ha; subst. 
-    exfalso; now apply H1.
-    inversion H12.
-    inversion H12.
+    exfalso; now apply H0.
+    inversion H10.
+    inversion H10.    
 Qed.
       
 (** Theorem 3. All typeable terms can reduce **)
 
-Theorem In_Value : forall e A, In e A -> Value e.
-Proof. intros e A HIn; induction HIn; auto. Qed.
 
 Theorem typeable_terms_reduce :
-  forall e1 A m, bidityping nil e1 m A -> (exists e2, red e1 e2) \/ Value e1.
+  forall e1 A m, bidityping nil e1 m A -> (exists e2, red e1 e2) \/ In e1 A.
 Proof.  
   intros e1 A m H.
   dependent induction H; eauto.
   - inversion H0.
   - left.
-    assert (Ha1 : (exists e2 : PExp, red t1 e2) \/ Value t1) by eauto.
+    assert (Ha1 : (exists e2 : PExp, red t1 e2) \/ In t1 (Fun A B)) by eauto.
     destruct Ha1.
     destruct H1; eauto.
-    assert (Ha2 : (exists e2, red t2 e2) \/ Value t2) by eauto.
+    assert (Ha2 : (exists e2, red t2 e2) \/ In t2 A) by eauto.
     destruct Ha2.
     destruct H2.
-    admit.
+    inversion H1; subst.
+    assert (Ha : red ( 
+    admit. (* *)
+    eauto.
     admit.
 Admitted.
 
